# Character Embedding

# 

$$h=1$$

$$\sum_{i=0}^n i^2 = \frac{(n^2+n)(2n+1)}{6}$$

$$\begin{pmatrix}a & b\\c & d\\\hline1 & 0\\0 & 1\end{pmatrix}$$

$$\left[\begin{matrix}1 & x & x^2 \\1 & y & y^2 \\1 & z & z^2 \\\end{matrix}\right]$$



$$f(x)=\left\{
\begin{aligned}
x & = & \cos(t) \\
y & = & \sin(t) \\
z & = & \frac xy
\end{aligned}
\right.$$

$$F^{HLLC} = \left\{
\begin{array}{rcl}
F_L       &      & {0      <      S_L}\\
F^*_L     &      & {S_L \leq 0 < S_M}\\
F^*_R     &      & {S_M \leq 0 < S_R}\\
F_R       &      & {S_R \leq 0}
\end{array} \right.$$

$$\mathop{\int\!\!\!\int}_S$$

$$\alpha A A \beta　B　\gamma　\Gamma　\delta　\Delta　\epsilon　E 
\varepsilon　　\zeta　Z　\eta　H　\theta　\Theta　\vartheta 
\iota　I　\kappa　K　\lambda　\Lambda　\mu　M　\nu　N 
\xi　\Xi　o　O　\pi　\Pi　\varpi　　\rho　P 
\varrho　　\sigma　\Sigma　\varsigma　　\tau　T　\upsilon　\Upsilon 
\phi　\Phi　\varphi　　\chi　X　\psi　\Psi　\omega　\Omega$$
$$
\begin{equation} 
a=1 
\tag{e2}
\end{equation}
$$



$$
\begin{equation} 
a=1 
\tag{e2}
\end{equation}
$$



$$
\begin{equation} 
a=1 
\tag{e2}
\end{equation}
$$
$$\eqref{e2}$$

$$\eqref{e2}$$

